ExistentialRules/ChaseSequence/Nontermination/Unblockability.lean
@@ -5,7 +5,7 @@ Released under Apache 2.0 license as described in the file LICENSE.
 
 module
 
-public import ExistentialRules.ChaseSequence.TreeDerivation
+public import ExistentialRules.ChaseSequence.Nontermination.HeadChoice
 
 /-!
 # Unblockability
@@ -19,15 +19,14 @@ public section
 
 variable {sig : Signature} [DecidableEq sig.P] [DecidableEq sig.C] [DecidableEq sig.V]
 
-/-- A trigger is unblockable if its result necessarily occurs in every derivation where the trigger is loaded. In the introducing paper this is called g-unblockable. -/
+/-- A trigger is unblockable for a given `HeadChoice` if, for every derivation, when the trigger is loaded in a node of the branch indicated by the `HeacChoice`, then the `HeadChoice` result of the trigger also occurs in that branch. In the introducing paper this is called g-unblockable. -/
 @[expose]
 def Trigger.unblockable
     {obs : ObsolescenceCondition sig}
     (trg : Trigger obs.toLaxObsolescenceCondition)
-    (i : Nat)
-    (lt : i < trg.rule.head.length)
-    (rules : RuleSet sig) : Prop :=
-  ∀ td : RegularTreeDerivation obs rules, ∀ node : td.NodeWithAddress, trg.loaded node.node.facts ->
-  ∃ node2 : td.NodeWithAddress, node ≼ node2 ∧
-  (trg.mapped_head[i]'(by grind)).toSet ⊆ node2.node.facts
+    (rules : RuleSet sig)
+    (hc : HeadChoice sig) : Prop :=
+  ∀ td : RegularTreeDerivation obs rules, ∀ node : (td.subderivation_for_headChoice hc).Node, trg.loaded node.val.facts ->
+  ∃ node2 : (td.subderivation_for_headChoice hc).Node, node ≼ node2 ∧
+  (trg.mapped_head[(hc trg).val]'(by grind)).toSet ⊆ node2.val.facts
 
