ExistentialRules/ChaseSequence/Nontermination/HeadChoice.lean
@@ -1,0 +1,105 @@
+/-
+Copyright 2026 Lukas Gerlach
+Released under Apache 2.0 license as described in the file LICENSE.
+-/
+
+module
+
+public import ExistentialRules.ChaseSequence.ChaseTree
+
+/-!
+# HeadChoice
+
+Here we define `HeadChoice`s, which are merely functions from triggers to head indices.
+We also define machinery to get a branch from a tree that corresponds to a given `HeadChoice`.
+-/
+
+public section
+
+/-- A `HeadChoice` is a function that maps each trigger to one of its head indices. -/
+abbrev HeadChoice (sig : Signature) [DecidableEq sig.P] [DecidableEq sig.C] [DecidableEq sig.V] := (trg : PreTrigger sig) -> Fin trg.rule.head.length
+
+variable {sig : Signature} [DecidableEq sig.P] [DecidableEq sig.C] [DecidableEq sig.V]
+
+/-- A `ChaseDerivationSkeleton` adheres to a `HeadChoice` if every origin uses the index that is the head choice of its trigger. -/
+@[expose]
+def ChaseDerivationSkeleton.adheres_to_headChoice
+    {obs : ObsolescenceCondition sig} {rules : RuleSet sig} {N : Type u} [CN : ChaseNode N obs rules]
+    (cd : ChaseDerivationSkeleton N obs rules) (hc : HeadChoice sig) : Prop :=
+  ∀ n ∈ cd, ∀ orig ∈ (CN.origin n), orig.snd = hc orig.fst.val
+
+namespace TreeDerivation
+
+variable {obs : ObsolescenceCondition sig} {rules : RuleSet sig} {N : Type u} [CN : ChaseNode N obs rules]
+
+/-- The generator function used to generate the tree branch corresponding to the given `HeadChoice`. -/
+def generator_for_headChoice (td : TreeDerivation N obs rules) (hc : HeadChoice sig) (n : td.NodeWithAddress) : Option td.NodeWithAddress :=
+  let next_trg_opt : Option (PreTrigger sig) := (n.childNodes.head?.bind (fun c => CN.origin c.node)).map (fun o => o.fst.val)
+  next_trg_opt.bind (fun trg => n.childNodes[hc trg]?)
+
+/-- The generator function produces a child node if it produces a value at all. -/
+theorem generator_for_headChoice_mem_childNodes {td : TreeDerivation N obs rules} {hc : HeadChoice sig} (n : td.NodeWithAddress) :
+    ∀ next ∈ td.generator_for_headChoice hc n, next ∈ n.childNodes := by
+  intro next next_mem
+  simp only [generator_for_headChoice] at next_mem; rw [Option.mem_def, Option.bind_eq_some_iff] at next_mem
+  rcases next_mem with ⟨_, _, next_mem⟩
+  rw [List.mem_iff_getElem?]
+  exact ⟨_, next_mem⟩
+
+/-- The generator function does not yield a new value if and only if the childNodes are empty. -/
+theorem generator_for_headChoice_eq_none_iff_childNodes_eq_nil {td : TreeDerivation N obs rules} {hc : HeadChoice sig} (n : td.NodeWithAddress) :
+    td.generator_for_headChoice hc n = none ↔ n.childNodes = [] := by
+  simp only [generator_for_headChoice]
+  cases n.childNodes.instDecidableEqNil.em with
+  | inl eq_nil => simp [eq_nil]
+  | inr ne_nil =>
+    have ne_nil' : n.subderivation.childNodes ≠ [] := by rw [n.childNodes_eq_childNodes]; simp [ne_nil]
+    rcases n.triggers_exist ne_nil' with ⟨trg, act, ingoing_eq, trg_eq, orig_eq⟩
+    apply iff_of_false _ ne_nil
+    intro contra
+    simp only [Option.bind_eq_none_iff] at contra
+    specialize contra trg.val (by
+      rw [List.head?_eq_some_head ne_nil, Option.bind_some]
+      suffices (ChaseNode.origin (n.childNodes.head ne_nil).node).map (fun o => o.fst.val.toPreTrigger) = ((ChaseNode.origin (n.childNodes.head ne_nil).node).map (fun o => o.fst)).map (fun trg => trg.val.toPreTrigger) by
+        rw [this, trg_eq]
+        . simp
+        . rw [n.childNodes_eq_childNodes]; apply List.mem_map_of_mem; simp
+      simp; rfl)
+
+    suffices (hc trg.val).val < (n.subderivation.childNodes.map (ChaseNode.ingoingFacts obs rules)).length by
+      apply Nat.not_le_of_lt this; rw [n.childNodes_eq_childNodes]; simp only [List.length_map]; rw [← List.getElem?_eq_none_iff]; exact contra
+    rw [ingoing_eq, List.length_map, PreTrigger.length_mapped_head]; exact (hc trg.val).isLt
+
+/-- This function generates the tree branch that corresponds to the given `HeadChoice`. -/
+def subderivation_for_headChoice (td : TreeDerivation N obs rules) (hc : HeadChoice sig) : ChaseDerivation N obs rules :=
+  td.generate_subderivation (NodeWithAddress.root td) (td.generator_for_headChoice hc) id td.generator_for_headChoice_mem_childNodes (by intro n; rw [generator_for_headChoice_eq_none_iff_childNodes_eq_nil]; rw [List.eq_nil_iff_length_eq_zero, List.eq_nil_iff_length_eq_zero, n.length_childNodes, n.subderivation.childNodes_eq]; simp)
+
+/-- The `subderivation_for_headChoice` is a branch, which follows since we use `TreeDerivation.generate_subderivation` to build it. -/
+theorem subderivation_for_headChoice_mem_branches {td : TreeDerivation N obs rules} {hc : HeadChoice sig} :
+  td.subderivation_for_headChoice hc ∈ td.branches := by apply td.generate_subderivation_mem_branches; rfl
+
+/-- The head of `subderivation_for_headChoice` is the root of the tree derivation. -/
+theorem head_subderivation_for_headChoice {td : TreeDerivation N obs rules} {hc : HeadChoice sig} :
+  (td.subderivation_for_headChoice hc).head = td.root := td.head_generate_subderivation
+
+end TreeDerivation
+
+namespace ChaseTree
+
+variable {obs : ObsolescenceCondition sig} {kb : KnowledgeBase sig} {N : Type u} [CN : ChaseNode N obs kb.rules]
+
+/-- This function generates the tree branch that corresponds to the given `HeadChoice`. -/
+@[expose]
+def subderivation_for_headChoice (ct : ChaseTree N obs kb) (hc : HeadChoice sig) : ChaseBranch N obs kb :=
+  let deriv := ct.toTreeDerivation.subderivation_for_headChoice hc
+  {
+    branch := deriv.branch,
+    isSome_head := deriv.isSome_head,
+    triggers_exist := deriv.triggers_exist,
+    triggers_active := deriv.triggers_active,
+    fairness := deriv.fairness,
+    database_first := by rw [TreeDerivation.head_subderivation_for_headChoice]; exact ct.database_first
+  }
+
+end ChaseTree
+
